proof/SimMod.v
@@ -33,13 +33,12 @@ Context `{SM: SimMem.class} {SS: SimSymb.class SM} {SU: Sound.class}.
     src: Mod.t;
     tgt: Mod.t;
     ss: SimSymb.t;
-    SMO:> SimMemOh.class;
   }.
 
   Definition to_msp (midx: Midx.t)
-             (skenv_link_src skenv_link_tgt: SkEnv.t) (sm: SimMem.t) (mp: t): ModSemPair.t
+             (skenv_link_src skenv_link_tgt: SkEnv.t) (sm: SimMem.t) (mp: t) SMO: ModSemPair.t
     := ModSemPair.mk (Mod.modsem (mp.(src)) midx skenv_link_src)
-                     (Mod.modsem (mp.(tgt)) midx skenv_link_tgt) mp.(ss) sm mp.(SMO).
+                     (Mod.modsem (mp.(tgt)) midx skenv_link_tgt) mp.(ss) sm (SMO).
 
   (* TODO: Actually, ModPair can have idx/ord and transfer it to ModSemPair. *)
   (* Advantage: We can unify ord at Mod state. *)
@@ -55,8 +54,8 @@ Context `{SM: SimMem.class} {SS: SimSymb.class SM} {SU: Sound.class}.
           (WFTGT: SkEnv.wf skenv_link_tgt)
           (SSLE: SimSymb.le mp.(ss) ss_link)
           (SIMSKENVLINK: SimSymb.sim_skenv sm_init_link ss_link skenv_link_src skenv_link_tgt),
-          <<SIMMSP: ModSemPair.sim
-                      (to_msp midx skenv_link_src skenv_link_tgt sm_init_link mp)>>).
+          exists SMO, <<SIMMSP: ModSemPair.sim
+                                  (to_msp midx skenv_link_src skenv_link_tgt sm_init_link mp SMO)>>).
   (* TODO: quantifying "exists SMO" here looks somewhat dirty... *)
   (* I would like to quantify it directly inside "sim_intro", but I need to put it here because *)
   (* I need to know "owned_heap" type which needs to know "skenv_link_src,tgt". *)
@@ -65,21 +64,6 @@ Context `{SM: SimMem.class} {SS: SimSymb.class SM} {SU: Sound.class}.
   (* TODO: the same goes for "state" too. *)
 
   (* Design: ModPair only has data, properties are stated in sim *)
-
-  Inductive simU {SMOS: SimMemOhs.class} (mp: t) (midx: Midx.t): Prop :=
-  | simU_intro
-      (SIMSK: SimSymb.wf mp.(ss))
-      (SKSRC: mp.(ss).(SimSymb.src) = (Mod.sk mp.(src)))
-      (SKTGT: mp.(ss).(SimSymb.tgt) = (Mod.sk mp.(tgt)))
-      (SIMMS: forall skenv_link_src skenv_link_tgt ss_link sm_init_link
-          (INCLSRC: SkEnv.includes skenv_link_src (Mod.sk mp.(src)))
-          (INCLTGT: SkEnv.includes skenv_link_tgt (Mod.sk mp.(tgt)))
-          (WFSRC: SkEnv.wf skenv_link_src)
-          (WFTGT: SkEnv.wf skenv_link_tgt)
-          (SSLE: SimSymb.le mp.(ss) ss_link)
-          (SIMSKENVLINK: SimSymb.sim_skenv sm_init_link ss_link skenv_link_src skenv_link_tgt),
-          <<SIMMSP: ModSemPair.simU (to_msp midx skenv_link_src skenv_link_tgt
-                                            sm_init_link mp)>>).
 
 End MODPAIR.
 End ModPair.
